cleaning up proofs and merging some files in

SP1Operations/U16ToU8OperationSafe.lean
@@ -4,7 +4,7 @@ import SP1Foundations
 namespace U16ToU8OperationSafe
 
 def constraints (I0 I1 I2 I3 I4 : BabyBear) :
-    Vector BabyBear 4 × List (SP1Constraint) :=
+    Vector BabyBear 4 × SP1ConstraintList :=
   let E0 := I0 - I2
   let E2 := E0 * 2005401601
   let E4 := I1 - I3
@@ -23,25 +23,13 @@ lemma outputVector_spec (I0 I1 I2 I3 I4 : BabyBear) :
     (v[0] + v[1] * 256 = I0) ∧ (v[2] + v[3] * 256 = I1) := by
   simp [mul_assoc]
 
--- def constraintSet
---     (I0 I1 I2 I3 I4 : BabyBear) :
---     (List SP1Constraint) :=
---   let E0 := I0 - I2
---   let E2 := E0 * 2005401601
---   let E4 := I1 - I3
---   let E6 := E4 * 2005401601
---   [
---     .send (.byte ByteOpcode.U8Range I2 E2 0) I4,
---     .send (.byte ByteOpcode.U8Range I3 E6 0) I4
---   ]
-
 def constraintProp (I0 I1 I2 I3 _I4 : BabyBear) : Prop :=
   I2 < 256 ∧ (I0 - I2) * 2005401601 < 256 ∧
     I3 < 256 ∧ (I1 - I3) * 2005401601 < 256
 
-lemma toProp_constraintSet_iff_constraintProp
+lemma constraints_iff_constraintProp
     (I0 I1 I2 I3 I4 : BabyBear) :
-    List.Forall SP1Constraint.toProp (constraints I0 I1 I2 I3 I4).2 ↔
+    (constraints I0 I1 I2 I3 I4).2.allHold ↔
       (I4 = 0 ∨ constraintProp I0 I1 I2 I3 I4) := by
   simp [constraintProp, constraints]
   by_cases hi4 : I4 = 0
@@ -54,9 +42,9 @@ def Spec (I0 I1 I2 I3 I4 : BabyBear) : Prop :=
 
 theorem spec_of_constraintSet
     (I0 I1 I2 I3 I4 : BabyBear)
-    (h : List.Forall SP1Constraint.toProp (constraints I0 I1 I2 I3 I4).2) :
+    (h : (constraints I0 I1 I2 I3 I4).2.allHold) :
     Spec I0 I1 I2 I3 I4 := by
-  rw [toProp_constraintSet_iff_constraintProp, constraintProp, or_iff_not_imp_left] at h
+  rw [constraints_iff_constraintProp, constraintProp, or_iff_not_imp_left] at h
   exact h
 
 section corrollary
@@ -64,29 +52,14 @@ section corrollary
 variable {I0 I1 I2 I3 I4 : BabyBear}
 
 lemma outputVector_bound (hi4 : I4 ≠ 0)
-    (h : List.Forall SP1Constraint.toProp (constraints I0 I1 I2 I3 I4).2) :
+    (h : (constraints I0 I1 I2 I3 I4).2.allHold) :
     ∀ x ∈ (constraints I0 I1 I2 I3 I4).1, x < 256 := by
   simpa using spec_of_constraintSet I0 I1 I2 I3 I4 h hi4
 
--- lemma outputVector_get_zero_bound (hi4 : I4 ≠ 0)
---     (h : List.Forall SP1Constraint.toProp (constraintSet I0 I1 I2 I3 I4)) :
---     (outputVector I0 I1 I2 I3 I4)[0] < 256 :=
---   outputVector_bound hi4 h _ <| by simp
-
--- lemma outputVector_get_one_bound (hi4 : I4 ≠ 0)
---     (h : List.Forall SP1Constraint.toProp (constraintSet I0 I1 I2 I3 I4)) :
---     (outputVector I0 I1 I2 I3 I4)[1] < 256 :=
---   outputVector_bound hi4 h _ <| by simp
-
--- lemma outputVector_get_two_bound (hi4 : I4 ≠ 0)
---     (h : List.Forall SP1Constraint.toProp (constraintSet I0 I1 I2 I3 I4)) :
---     (outputVector I0 I1 I2 I3 I4)[2] < 256 :=
---   outputVector_bound hi4 h _ <| by simp
-
--- lemma outputVector_get_three_bound (hi4 : I4 ≠ 0)
---     (h : List.Forall SP1Constraint.toProp (constraintSet I0 I1 I2 I3 I4)) :
---     (outputVector I0 I1 I2 I3 I4)[3] < 256 :=
---   outputVector_bound hi4 h _ <| by simp
+lemma outputVector_bound' (hi4 : I4 ≠ 0)
+    (h : (constraints I0 I1 I2 I3 I4).2.allHold)
+    (i : Fin 4) : (constraints I0 I1 I2 I3 I4).1[i] < 256 :=
+  outputVector_bound hi4 h _ (Vector.mem_of_getElem rfl)
 
 end corrollary
 
