SP1Operations/BitWiseU16Operation.lean
@@ -1,0 +1,73 @@
+import SP1Foundations
+import SP1Operations.MemoryConsistency
+import SP1Operations.U16toU8OperationUnsafe
+import SP1Operations.BitwiseOperation
+import LeanRV32D.RiscvRegs
+
+open LeanRV32D.Functions
+
+structure BitwiseU16Operation where
+  b_low_bytes : U16toU8Operation
+  c_low_bytes : U16toU8Operation
+  bitwise_operation : BitwiseOperation
+
+namespace BitwiseU16Operation
+
+def constraint
+  (b : Word BabyBear)
+  (cc : Word BabyBear)
+  (cols : BitwiseU16Operation)
+  (opcode : BabyBear)
+  (is_real : BabyBear)
+  : Word BabyBear × List SP1Constraint :=
+  let E0 : BabyBear := is_real - 1
+  let E2 : BabyBear := is_real * E0
+
+  let ⟨V0, CS0⟩ := U16ToU8OperationUnsafe.constraints
+    #v[b[0], b[1]]
+    { low_bytes :=
+        #v[cols.b_low_bytes.low_bytes[0]
+        , cols.b_low_bytes.low_bytes[1]
+        ]
+    }
+  -- We will have our own syntax to pattern match
+  -- Vector BabyBear WORD_BYTE_SIZE
+  let E4 : BabyBear := V0[0]
+  let E5 : BabyBear := V0[1]
+  let E6 : BabyBear := V0[1]
+  let E7 : BabyBear := V0[1]
+
+  let ⟨V1, CS1⟩ := U16ToU8OperationUnsafe.constraints
+    #v[cc[0], cc[1]]
+    { low_bytes :=
+        #v[cols.c_low_bytes.low_bytes[0]
+        , cols.c_low_bytes.low_bytes[1]
+        ]
+    }
+  -- We will have our own syntax to pattern match
+  -- Vector BabyBear WORD_BYTE_SIZE
+  let E8 : BabyBear := V0[0]
+  let E9 : BabyBear := V0[1]
+  let E10 : BabyBear := V0[1]
+  let E11 : BabyBear := V0[1]
+
+  let E12 : BabyBear := cols.bitwise_operation.result[1] * 256
+  let E14 : BabyBear := E8 + E12
+  let E16 : BabyBear := cols.bitwise_operation.result[3] * 256
+  let E18 : BabyBear := E10 + E16
+
+  ⟨#v[E14, E18],
+  [ .assertZero E2
+  ] ++ CS0 ++ CS1 ++ (BitwiseOperation.constraints
+      #v[E4, E5, E6, E7]
+      #v[E8, E9, E10, E11]
+      { result :=
+          #v[cols.bitwise_operation.result[0]
+          ,  cols.bitwise_operation.result[1]
+          ,  cols.bitwise_operation.result[2]
+          ,  cols.bitwise_operation.result[3]
+          ] }
+      opcode
+      is_real)⟩
+
+end BitwiseU16Operation
